ifc/rules.v
@@ -19,6 +19,10 @@ Local Open Scope logic.
 Definition ioverridePost{A: Type}(Q: A -> environ -> mpred)(R : A -> ret_assert): A -> ret_assert :=
   fun (x: A) => (overridePost (Q x) (R x)).
 
+Definition overridePostClsf{A C: Type}(Q: A -> C)(R: A -> exitkind -> option val -> C)
+: A -> exitkind -> option val -> C
+:= fun (x: A) (ek: exitkind) (vl: option val) => if eq_dec ek EK_normal then Q x else R x ek vl.
+
 Ltac split_ifc_hyps :=
   repeat match goal with
   | H: ifc_def _ _ _ _ _ _ _ _ _ |- _ =>
@@ -27,10 +31,12 @@ Ltac split_ifc_hyps :=
       destruct H as [Hs Hi]
   end.
 
-Lemma star_seq_inv: forall ge e1 te1 e3 te3 h t m1 m3 c,
-  star ge (State e1 te1 (Kseq (Ssequence h t) :: c)) m1 (State e3 te3 c) m3 ->
-  exists e2 te2 m2, star ge (State e1 te1 (Kseq h :: Kseq t :: c)) m1 (State e2 te2 (Kseq t :: c)) m2
-                 /\ star ge (State e2 te2 (Kseq t :: c)) m2 (State e3 te3 c) m3.
+Lemma star_seq_inv: forall ge e1 te1 e3 te3 h t m1 m3 c ek3 vl3,
+  star ge (State e1 te1 (Kseq (Ssequence h t) :: c)) m1 (State e3 te3 (exit_cont ek3 vl3 c)) m3 ->
+  exists e2 te2 m2 ek2 vl2,
+  star ge (State e1 te1 (Kseq h :: Kseq t :: c)) m1 (State e2 te2 (exit_cont ek2 vl2 (Kseq t :: c))) m2
+ /\ star ge (State e2 te2 (exit_cont ek2 vl2 (Kseq t :: c))) m2 (State e3 te3 (exit_cont ek3 vl3 c)) m3
+ /\ (ek2 = EK_normal \/ (ek2 = ek3 /\ vl2 = vl3)).
 Proof.
 (* old proof
   intros. inverts H as Step Star. inverts Step as Step.
@@ -57,14 +63,32 @@ Definition iprop{A: Type}(P: pre_assert): A -> pre_assert := fun (_: A) => P.
 Definition inormal_ret_assert{A: Type}(P: A -> environ -> mpred): A -> ret_assert :=
   fun (x: A) => normal_ret_assert (P x).
 
+Definition normalPostClsf{A Loc: Type}(Q: A -> Loc -> label)
+: A -> exitkind -> option val -> Loc -> label
+:= fun (x: A) (ek: exitkind) (vl: option val) => if eq_dec ek EK_normal then Q x else bot.
+
+Lemma star_null:
+  forall ge s s' m m',
+  star ge s m s' m' ->
+  forall e te c e' te', s = (State e te c) /\
+  s' = (State e' te' c) ->
+  e' = e /\ te' = te /\ m' = m.
+Proof.
+Admitted. (* TODO: Not sure that this is true: if I have a while loop for instance,
+what does the semantics do? *)
+
 Section RULES.
 Context {Espec : OracleKind}.
 Context {CS: compspecs}.
 
+Arguments stack_lo_equiv _ _ _ _: simpl never.
+
 Lemma ifc_seq{T: Type}:
-  forall Delta (P1 P2: T -> environ -> mpred) (P3: T -> ret_assert) h t
-    (N1 N2 N3: T -> stack_clsf) (A1 A2 A3: T -> heap_clsf),
-  ifc_def T Delta P1 N1 A1 h (ioverridePost P2 P3) N2 A2 ->
+  forall Delta h t
+    (P1 P2: T -> environ -> mpred) (P3: T -> ret_assert)
+    (N1 N2: T -> stack_clsf) (N3: T -> ret_stack_clsf)
+    (A1 A2: T -> heap_clsf) (A3: T -> ret_heap_clsf),
+  ifc_def T Delta P1 N1 A1 h (ioverridePost P2 P3) (overridePostClsf N2 N3) (overridePostClsf A2 A3) ->
   ifc_def T (update_tycon Delta h) P2 N2 A2 t P3 N3 A3 ->
   ifc_def T Delta P1 N1 A1 (Ssequence h t) P3 N3 A3.
 Proof.
@@ -72,25 +96,61 @@ Proof.
   - intro. apply* semax_seq.
   - unfold ifc_core, simple_ifc in *.
     intros x x' ge e1 e1' e3 e3' te1 te1' te3 te3' m1 m1' m3 m3' c'.
-    intros Sat1 Sat1' SE1 HE1 Star1 Star1'.
-    apply star_seq_inv in Star1. destruct Star1 as [e2 [te2 [m2 [Star1 Star2]]]].
-    apply star_seq_inv in Star1'. destruct Star1' as [e2' [te2' [m2' [Star1' Star2']]]].
-    edestruct H1i as [SE2 HE2].
+    introv Sat1 Sat1' SE1 HE1 Star1 Star1'.
+    apply star_seq_inv in Star1.
+    apply star_seq_inv in Star1'.
+    destruct Star1  as [e2  [te2  [m2  [ek2  [vl2  [Star1  [Star2  EE ]]]]]]].
+    destruct Star1' as [e2' [te2' [m2' [ek2' [vl2' [Star1' [Star2' EE']]]]]]].
+    edestruct H1i as [Eek [Nvl [SE2 HE2]]].
     + eapply Sat1.
     + eapply Sat1'.
     + apply* stack_lo_equiv_change_cmd.
     + exact HE1.
     + exact Star1.
     + exact Star1'.
-    + clear H1i. eapply H2i.
-      * pose proof (VST_sound _ _ _ _ (Kseq t :: c') (H1s x)) as C. unfold ioverridePost in C.
-        erewrite <- VST_overridePost_to_state_pred. apply* C.
-      * pose proof (VST_sound _ _ _ _ (Kseq t :: c') (H1s x')) as C. unfold ioverridePost in C.
-        erewrite <- VST_overridePost_to_state_pred. apply* C.
-      * apply* stack_lo_equiv_change_cmd.
-      * exact HE2.
-      * exact Star2.
-      * exact Star2'.
+    + clear H1i. subst ek2'.
+      destruct ek2.
+      { pose proof (VST_sound _ _ _ _ EK_normal vl2 (Kseq t :: c') (H1s x)) as C.
+        pose proof (VST_sound _ _ _ _ EK_normal vl2' (Kseq t :: c') (H1s x')) as C'.
+        unfold ioverridePost in C, C'.
+        erewrite VST_overridePost_to_state_pred in C, C'.
+        eapply H2i.
+        * edestruct C as [? ?]; eassumption.
+        * edestruct C' as [? ?]; eassumption.
+        * apply* stack_lo_equiv_change_cmd.
+        * exact HE2.
+        * exact Star2.
+        * exact Star2'. }
+      { unfold overridePostClsf in *; simpl in *.
+        destruct EE  as [? | [? ?]]; [discriminate | subst ek  vl2  ].
+        destruct EE' as [? | [? ?]]; [discriminate | subst ek' vl2' ].
+        refine (conj eq_refl (conj Nvl _)).
+        simpl exit_cont in *.
+        eapply star_null in Star2 ; [ | eapply (conj eq_refl eq_refl) ].
+        eapply star_null in Star2'; [ | eapply (conj eq_refl eq_refl) ].
+        destruct Star2  as [? [? ?]]; subst e2  te2  m2 .
+        destruct Star2' as [? [? ?]]; subst e2' te2' m2'.
+        apply (conj SE2 HE2). }
+      { unfold overridePostClsf in *; simpl in *.
+        destruct EE  as [? | [? ?]]; [discriminate | subst ek  vl2  ].
+        destruct EE' as [? | [? ?]]; [discriminate | subst ek' vl2' ].
+        refine (conj eq_refl (conj Nvl _)).
+        simpl exit_cont in *.
+        eapply star_null in Star2 ; [ | eapply (conj eq_refl eq_refl) ].
+        eapply star_null in Star2'; [ | eapply (conj eq_refl eq_refl) ].
+        destruct Star2  as [? [? ?]]; subst e2  te2  m2 .
+        destruct Star2' as [? [? ?]]; subst e2' te2' m2'.
+        apply (conj SE2 HE2). }
+      { unfold overridePostClsf in *; simpl in *.
+        destruct EE  as [? | [? ?]]; [discriminate | subst ek  vl2  ].
+        destruct EE' as [? | [? ?]]; [discriminate | subst ek' vl2' ].
+        refine (conj eq_refl (conj Nvl _)).
+        simpl exit_cont in *.
+        eapply star_null in Star2 ; [ | eapply (conj eq_refl eq_refl) ].
+        eapply star_null in Star2'; [ | eapply (conj eq_refl eq_refl) ].
+        destruct Star2  as [? [? ?]]; subst e2  te2  m2 .
+        destruct Star2' as [? [? ?]]; subst e2' te2' m2'.
+        apply (conj SE2 HE2). }
 Grab Existential Variables. exact nil. exact nil. exact nil. exact nil.
 Qed.
 
@@ -107,41 +167,38 @@ Proof.
 Qed.
 (* "Search (?h :: ?t = ?t)." only gives the above lemma, so probably that doesn't exist already *)
 
-Lemma star_null:
-  forall ge s s' m m',
-  star ge s m s' m' ->
-  forall e te c e' te', s = (State e te c) /\
-  s' = (State e' te' c) ->
-  e' = e /\ te' = te /\ m' = m.
-Proof.
-Admitted. (* TODO: Not sure that this is true: if I have a while loop for instance,
-what does the semantics do? *)
- 
-Lemma star_skip_elim:
+Lemma star_skip_elim00:
   forall ge e te c m e' te' m',
   star ge (State e te (Kseq Sskip :: c)) m (State e' te' c) m' ->
   e' = e /\ te' = te /\ m' = m.
 Proof.
-  intros.
-  inverts H as Step Star; subst.
-  - eapply blah in Step. inversion Step.
+  intros. unfold star, corestep_star in H. destruct H as [n H].
+  destruct n as [| n].
+  - inversion H. subst. exfalso. eapply blah. eassumption.
   - remember (State e te (Kseq Sskip :: c)) as s.
     remember (State e' te' c) as s'.
-    induction Step; subst; inverts Heqs.
 (* ugh. from Step and Star conclude star from c to c,
         use that to conclude the equalities. *)
 Admitted.
-  
+
+(* TODO not sure if this holds *)
+Lemma star_skip_elim: forall ge e1 te1 k m1 e2 te2 m2 ek vl,
+  star ge (State e1 te1 (Kseq Sskip :: k)) m1
+          (State e2 te2 (exit_cont ek vl k)) m2 ->
+  e1 = e2 /\ te1 = te2 /\ m1 = m2 /\ ek = EK_normal /\ vl = None.
+Admitted.
+
 Lemma ifc_skip{T: Type}:
   forall Delta P N A,
-  ifc_def T Delta P N A Sskip (inormal_ret_assert P) N A.
+  ifc_def T Delta P N A Sskip (inormal_ret_assert P) (normalPostClsf N) (normalPostClsf A).
 Proof.
   intros. unfold ifc_def, ifc_core, simple_ifc. split.
   - intro x. apply semax_skip.
   - introv Sat Sat' SE HE Star Star'.
-    eapply star_skip_elim in Star. destruct Star as [? [? ?]]; subst.
-    eapply star_skip_elim in Star'. destruct Star' as [? [? ?]]; subst.
-    split.
+    eapply star_skip_elim in Star. destruct Star as [? [? [? [? ?]]]]; subst.
+    eapply star_skip_elim in Star'. destruct Star' as [? [? [? [? ?]]]]; subst.
+    refine (conj eq_refl (conj _ (conj _ _))).
+    + unfold same_Noneness. left. auto.
     + unfold stack_lo_equiv.
       unfold stack_lo_equiv in SE.
       apply SE.
@@ -157,7 +214,7 @@ Admitted.
 Lemma ifc_ifthenelse: forall {T: Type} (Delta: tycontext) 
   (P: T -> pre_assert) (N: T -> stack_clsf) (A: T -> heap_clsf)
   (b: expr) (c1 c2: statement)
-  (P': T -> ret_assert) (N': T -> stack_clsf) (A': T -> heap_clsf),
+  (P': T -> ret_assert) (N': T -> ret_stack_clsf) (A': T -> ret_heap_clsf),
   bool_type (typeof b) = true ->
   ifc_def T Delta (iand P (iprop (local (`(typed_true  (typeof b)) (eval_expr b))))) N A c1 P' N' A' ->
   ifc_def T Delta (iand P (iprop (local (`(typed_false (typeof b)) (eval_expr b))))) N A c2 P' N' A' ->
@@ -173,20 +230,35 @@ Proof.
 Admitted.
 
 Lemma ifc_return{T: Type}:
-  forall Delta R N A ret,
+  forall Delta (R: T -> ret_assert) (N: T -> ret_stack_clsf) (A: T -> ret_heap_clsf)
+        (retExpr: option expr) (retVal: option val),
+(* TODO this is an equality between two things of type "environ -> mpred", probably not what we want *)
+  (cast_expropt retExpr (ret_type Delta)) = `retVal ->
   ifc_def T Delta
-          (fun x => (tc_expropt Delta ret (ret_type Delta) &&
-                    `( R x EK_return : option val -> environ -> mpred)
-                     (cast_expropt ret (ret_type Delta)) id)) N A
-          (Sreturn ret)
-          (fun x => R x) N A.
+          (fun (x: T) => tc_expropt Delta retExpr (ret_type Delta) &&
+                         R x EK_return retVal)
+          (fun (x: T) => N x EK_return retVal)
+          (fun (x: T) => A x EK_return retVal)
+          (Sreturn retExpr)
+          R N A.
 Proof.
   intros. unfold ifc_def, ifc_core, simple_ifc. split.
-  - intro x. apply semax_return.
+  - intro x. 
+    pose proof (semax_return Delta (R x) retExpr) as C.
+    assert (forall rho, cast_expropt retExpr (ret_type Delta) rho = retVal) as H'. {
+      rewrite H. intro. reflexivity.
+    }
+    unfold liftx in C. unfold lift_uncurry_open in C. simpl in C. unfold lift in C.
+    assert ((fun x0 : environ =>
+       tc_expropt Delta retExpr (ret_type Delta) x0 &&
+       R x EK_return (cast_expropt retExpr (ret_type Delta) x0) x0) =
+       (fun x0 : environ =>
+       tc_expropt Delta retExpr (ret_type Delta) x0 &&
+       R x EK_return retVal x0)) as E. {
+      extensionality. f_equal. f_equal. apply H'.
+    }
+    rewrite E in C. clear E. apply C.
   - introv Sat Sat' SE HE Star Star'.
-    inverts Star as Step Star.
-    + exfalso. eapply blah. eapply Step.
-    + inversion Step. subst.
     (* TODO... *)
 Admitted.
 
@@ -201,12 +273,12 @@ Proof.
   - intro. apply semax_pre with (P' := P1' x); auto.
   - unfold ifc_core, simple_ifc in *.
     introv Sat Sat' SE HE. 
-    pose proof (VST_pre_to_state_pred_commutes_imp' _ _ _ (E x) _ _ _ Sat) as Sat0.
-    pose proof (VST_pre_to_state_pred_commutes_imp' _ _ _ (E x') _ _ _ Sat') as Sat'0.
-    pose proof (VST_pre_to_state_pred_commutes_imp _ _ (Imp x) _ _ _ Sat) as Sat00.
-    pose proof (VST_pre_to_state_pred_commutes_imp _ _ (Imp x') _ _ _ Sat') as Sat'00.
-    apply VST_indep_state_pred in Sat00. destruct Sat00 as [LeA LeN].
-    apply VST_indep_state_pred in Sat'00. destruct Sat'00 as [LeA' LeN'].
+    pose proof (VST_to_state_pred_commutes_imp' _ _ _ (E x) _ _ _ Sat) as Sat0.
+    pose proof (VST_to_state_pred_commutes_imp' _ _ _ (E x') _ _ _ Sat') as Sat'0.
+    pose proof (VST_to_state_pred_commutes_imp _ _ (Imp x) _ _ _ Sat) as Sat00.
+    pose proof (VST_to_state_pred_commutes_imp _ _ (Imp x') _ _ _ Sat') as Sat'00.
+    rewrite VST_indep_state_pred in Sat00. destruct Sat00 as [LeA LeN].
+    rewrite VST_indep_state_pred in Sat'00. destruct Sat'00 as [LeA' LeN'].
     apply* Hi.
     + apply* weaken_stack_lo_equiv.
     + apply* weaken_heap_lo_equiv.
@@ -245,12 +317,14 @@ Lemma bigstep_null:
     forall ge e te e' te' m m' c',
     star ge (State e te []) m (State e' te' c') m' ->
     m' = m /\ e' = e /\ te' = te /\ c' = [].
+Admitted. (*
 Proof.
   intros.
   inversion H; subst.
   - auto.
   - inversion H0.
 Qed.
+*)
 
 Lemma bigstep_sassign:
     forall ge e te e1 e2 m e' te' m' k, 
@@ -261,6 +335,7 @@ Lemma bigstep_sassign:
       Clight.eval_expr ge e te m e2 v2 /\
       assign_loc ge (typeof e1) m loc ofs v1 m' /\
       Cop.sem_cast v2 (typeof e2) (typeof e1) m = Some v1.
+Admitted. (*
 Proof.
   intros.
   inverts H as Step Star.
@@ -271,6 +346,7 @@ Proof.
     destruct Star as [? [? ?]]; subst.
   do 4 eexists. eauto.
 Qed.
+*)
 
 Lemma ifc_store{T: Type}:
     forall Delta sh n (p: T -> val) P Q R (e1 e2 : expr)
@@ -294,16 +370,17 @@ Lemma ifc_store{T: Type}:
       (forall x, ENTAIL Delta, PROPx (P x) (LOCALx (Q x) (SEPx (R x))) |--
                  !! (clsf_expr (N x) true e1 = Some (l1 x) /\
                      clsf_expr (N x) false e2 = Some (l2 x))) ->
-      ifc [x: T] Delta |--
-        (|>PROPx (P x) (LOCALx (Q x) (SEPx (R x))))
-        (N x)
-        (A x)
+      ifc_def T Delta
+        (fun x => (|>PROPx (P x) (LOCALx (Q x) (SEPx (R x)))))
+        N
+        A
         (Sassign e1 e2)
-        (normal_ret_assert (PROPx (P x)
-                           (LOCALx (Q x)
-                           (SEPx (replace_nth n (R x) (data_at sh t (v_new x) (p x)))))))
-        (N x)
-        (fun loc => if heap_loc_eq_val loc (p x) then lub (l1 x) (l2 x) else A x loc).
+        (fun x => (normal_ret_assert (PROPx (P x)
+                                     (LOCALx (Q x)
+                                     (SEPx (replace_nth n (R x) (data_at sh t (v_new x) (p x))))))))
+        (normalPostClsf N)
+        (normalPostClsf (fun x loc =>
+           if heap_loc_eq_val loc (p x) then lub (l1 x) (l2 x) else A x loc)).
 Proof.
   introv EqT ByVal Volatile GetR Eval1 Eval2 JM Wsh Tc Ifc.
   unfold ifc_def. split.
@@ -311,6 +388,7 @@ Proof.
     eapply semax_SC_field_store_without_paths; eauto.
   - unfold ifc_core. unfold simple_ifc.
     introv Sat Sat' SE HE Star Star'.
+(*
     eapply bigstep_sassign in Star.
     destruct Star as [loc [ofs [v1 [v2 [HEval1 [HVolatile [HEval2 [HALoc HCast]]]]]]]].
     eapply bigstep_sassign in Star'.
@@ -318,6 +396,7 @@ Proof.
     (* OK now have semantic information about the effect
        of the store statement which we need to use to
        prove the infoflow conditions *)
+*)
 Admitted.
 
 End RULES.
